ulib/FStar.Tactics.Print.fst
@@ -4,6 +4,7 @@ open FStar.Reflection
 open FStar.Tactics.Effect
 open FStar.Tactics.Builtins
 open FStar.Tactics.Derived
+open FStar.Tactics.NamedView
 
 (* FIXME *)
 let namedv_to_string x = "namedv_to_string IOU"
@@ -22,6 +23,9 @@ let rec print_list_aux (f:'a -> Tac string) (xs:list 'a) : Tac string =
 private
 let print_list (f:'a -> Tac string) (l:list 'a) : Tac string =
    "[" ^ print_list_aux f l ^ "]"
+
+let named_binder_to_string (n : named_binder) : Tac string =
+  unseal n.ppname
 
 let rec universe_to_ast_string (u:universe) : Tac string =
   match inspect_universe u with
@@ -44,15 +48,15 @@ let rec term_to_ast_string (t:term) : Tac string =
   | Tv_UInst fv us ->
     "Tv_UInst" ^ paren (fv_to_string fv ^ ", " ^ universes_to_ast_string us)
   | Tv_App hd (a, _) -> "Tv_App " ^ paren (term_to_ast_string hd ^ ", " ^ term_to_ast_string a)
-  | Tv_Abs x e -> "Tv_Abs " ^ paren (binder_to_string x ^ ", " ^ term_to_ast_string e)
-  | Tv_Arrow x c -> "Tv_Arrow " ^ paren (binder_to_string x ^ ", " ^ comp_to_ast_string c)
+  | Tv_Abs x e -> "Tv_Abs " ^ paren (named_binder_to_string x ^ ", " ^ term_to_ast_string e)
+  | Tv_Arrow x c -> "Tv_Arrow " ^ paren (named_binder_to_string x ^ ", " ^ comp_to_ast_string c)
   | Tv_Type u -> "Type" ^ paren (universe_to_ast_string u)
-  | Tv_Refine x sort e -> "Tv_Refine " ^ paren (bv_to_string x ^ ", " ^ term_to_ast_string sort ^", " ^ term_to_ast_string e)
+  | Tv_Refine x e -> "Tv_Refine " ^ paren (named_binder_to_string x ^ ", " ^ term_to_ast_string e)
   | Tv_Const c -> const_to_ast_string c
   | Tv_Uvar i _ -> "Tv_Uvar " ^ string_of_int i
-  | Tv_Let recf _ x _ e1 e2 ->
+  | Tv_Let recf _ x e1 e2 ->
            "Tv_Let " ^ paren (string_of_bool recf ^ ", " ^
-                              bv_to_string x ^ ", " ^
+                              named_binder_to_string x ^ ", " ^
                               term_to_ast_string e1 ^ ", " ^
                               term_to_ast_string e2)
   | Tv_Match e ret_opt brs ->
